# Euler's Theorem
## Proof
MacLaurin's Series Expansion
$$\cos \theta x=1-\frac{(x\theta)^2}{2!}+\frac{(x\theta)^4}{4!}-\dots$$
$$i\sin \theta x=ix\theta-i\frac{(x\theta)^3}{3!}+i\frac{(x\theta)^5}{5!}-\dots$$

$$\cos\theta x + i\sin\theta x = 1+ix\theta-\frac{(x\theta)^2}{2!}-i\frac{(x\theta)^3}{3!}+\frac{(x\theta)^4}{4!}+i\frac{(x\theta)^5}{5!}-\dots$$
___
$$e^{i\theta x}=1+ i\theta x + \frac{i^2\theta^2 x^2}{2!} + \frac{i^3\theta^3 x^3}{3!} + \frac{i^4\theta^4 x^4}{4!} + \frac{i^5\theta^5 x^5}{5!}+\dots$$
$$e^{i\theta x}=1+ i\theta x - \frac{\theta^2 x^2}{2!} - i\frac{\theta^3 x^3}{3!} + \frac{\theta^4 x^4}{4!} + i\frac{\theta^5 x^5}{5!}-\dots$$


