# $$a+\frac{1}{a}\equiv$$
## Derivation
#Todo 
$$\frac 1 a(a^2+\frac 1 a) \equiv$$
$$\frac 1 a(a^2+\frac 1 a) \equiv$$

# $$a-\frac{1}{a}\equiv\left(1-\frac{1}{a}\right)\left(a+1\right)$$
## Derivation
$$\frac{1}{a}(a^2-1)\equiv a-\frac{1}{a}$$
$$\frac{1}{a}(a-1)(a+1)\equiv a-\frac{1}{a}$$
$$\left(1-\frac{1}{a}\right)\left(a+1\right)\equiv a-\frac{1}{a}$$

# $$ab-\frac{1}{ab}$$
## $$ab-\frac{1}{ab}\equiv(b-\frac1 a)(a + \frac1 b)$$
### Derivation
$$\frac{1}{ab}(a^2b^2-1)\equiv$$
$$\frac{1}{ab}(ab-1)(ab+1)\equiv$$
$$\frac{(ab-1)}{a}\frac{(ab+1)}{b}\equiv$$
$$(b-\frac1 a)(a+\frac1 b)\equiv$$

## $$ab-\frac{1}{ab}\equiv\frac 1 2 \left(a-\frac{1}{a}\right)\left(b+\frac{1}{b}\right) + \frac 1 2 \left(a+\frac{1}{a}\right)\left(b-\frac{1}{b}\right)$$
### Derivation
$$\frac{1}{2}\left(2ab-\frac2 {ab}\right)\equiv\dots$$
$$\frac{1}{2}\left(2ab-\frac2 {ab}+\frac{a}{b}-\frac a b + \frac b a - \frac b a\right)\equiv\dots$$
$$\frac 1 2 \left(ab + \frac a b - \frac b a - \frac 1 {ab} \right)+\frac 1 2\left(ab - \frac a b + \frac b a - \frac 1 {ab} \right)\equiv\dots$$
$$\frac 1 2 \left(a-\frac{1}{a}\right)\left(b+\frac{1}{b}\right) + \frac 1 2 \left(a+\frac{1}{a}\right)\left(b-\frac{1}{b}\right)\equiv\dots$$

## $$ab+\frac{1}{ab}\equiv$$

### Derivation
#Todo
$$\frac{1}{2}\left(2ab+\frac2 {ab} \right)\equiv$$
$$\frac{1}{2}\left(2ab+\frac2 {ab}+\frac{a}{b}-\frac a b + \frac b a - \frac b a\right)\equiv\dots$$
$$\frac 1 2 \left(ab + \frac a b - \frac b a + \frac 1 {ab} \right)+\frac 1 2\left(ab - \frac a b + \frac b a + \frac 1 {ab} \right)\equiv\dots$$
$$\frac 1 2 \left(a-\frac{1}{a}\right)\left(b+\frac{1}{b}\right) + \frac 1 2 \left(a+\frac{1}{a}\right)\left(b-\frac{1}{b}\right)\equiv\dots$$